Environments.v
@@ -1,191 +1,360 @@
-Require Import Coq.Strings.String.
+Require Import Coq.Strings.String Coq.Lists.List.
 Require Import SGA.Common.
 
-Create HintDb types discriminated.
-Hint Extern 1 => unfold not in *: types.
+Import ListNotations.
 
-Record fenv {Key Value: Type} :=
-  { fn :> Key -> Value -> Prop;
-    uniq: forall k v v', fn k v -> fn k v' -> v = v' }.
+Inductive member {K: Type}: K -> list K -> Type :=
+| MemberHd: forall k sig, member k (k :: sig)
+| MemberTl: forall k k' sig, member k sig -> member k (k' :: sig).
 
-Arguments fenv: clear implicits.
-Hint Resolve @uniq : types.
-
-Definition fenv_nil {Key Value: Type} : fenv Key Value :=
-  {| fn k v := False;
-     uniq := ltac:(cbv in *; tauto) |}.
-
-Definition fenv_add {Key Value: Type} (env: fenv Key Value) (k: Key) (v: Value) : fenv Key Value.
-  refine {| fn := (fun k' v' => (k = k' /\ v = v') \/ (k <> k' /\ env.(fn) k' v')) |};
-    abstract (destruct env; intuition (subst; eauto with types)).
+Definition mdestruct {K sig} {k: K} (m: member k sig)
+  : match sig return member k sig -> Type with
+    | [] => fun m => False
+    | k' :: sig => fun m => ({ eqn: k = k' & m = eq_rect _ _ (fun _ => MemberHd k sig) _ eqn m } +
+                        { m': member k sig & m = MemberTl k k' sig m' })%type
+    end m.
+  destruct m; cbn.
+  - left; exists eq_refl; eauto.
+  - right; eauto.
 Defined.
 
-Definition fenv_le {Key Value: Type} (cmp : Value -> Value -> Prop) (Gamma Gamma': fenv Key Value) :=
-  forall k v, Gamma k v -> exists v', Gamma' k v' /\ cmp v v'.
+Fixpoint mem {K} `{EqDec K} (k: K) sig {struct sig} : member k sig + (member k sig -> False).
+  destruct sig.
+  - right; inversion 1.
+  - destruct (eq_dec k k0) as [Heq | Hneq].
+    + subst. left. apply MemberHd.
+    + destruct (mem _ _ k sig) as [m | ].
+      * left. apply MemberTl. exact m.
+      * right. inversion 1; congruence.
+Defined.
 
-Class Env {K V: Type}: Type :=
-  { env_t: Type;
-    env_nil: env_t;
-    getenv: env_t -> K -> option V;
-    putenv: env_t -> K -> V -> env_t;
-    getenv_nil: forall k, getenv env_nil k = None;
-    get_put_eq: forall ev k v, getenv (putenv ev k v) k = Some v;
-    get_put_neq: forall ev k k' v, k <> k' -> getenv (putenv ev k v) k' = getenv ev k';
-    get_put_Some: forall ev k k' v v',
-        getenv (putenv ev k v) k' = Some v' <->
-        k = k' /\ v = v' \/ k <> k' /\ getenv ev k' = Some v';
-    get_put_None: forall ev k k' v,
-        getenv (putenv ev k v) k' = None <->
-        k <> k' /\ getenv ev k' = None
-  }.
-Arguments Env : clear implicits.
-Arguments env_t {_ _}.
+Fixpoint find {K} (fn: K -> bool) sig {struct sig} : option { k: K & member k sig }.
+  destruct sig.
+  - right.
+  - destruct (fn k) eqn:?.
+    + left. eexists. apply MemberHd.
+    + destruct (find _ fn sig) as [ (k' & m) | ].
+      * left. eexists. apply MemberTl. eassumption.
+      * right.
+Defined.
 
-Instance EqEnv {K V: Type} (eqdec: forall k k': K, {k = k'} + {k <> k'}) : Env K V.
+Fixpoint assoc {K1 K2: Type} `{EqDec K1}
+         (k1: K1) sig {struct sig} : option { k2: K2 & member (k1, k2) sig }.
 Proof.
-  refine ({| env_t := list (K * V);
-             env_nil := nil;
-             getenv e k :=
-               match List.find (fun '(k', v) => if eqdec k k' then true else false) e with
-               | Some (_, v) => Some v
-               | None => None
-               end;
-             putenv e k v := cons (k, v) e |}); intros.
-  - abstract (reflexivity).
-  - abstract (cbn; destruct eqdec; congruence).
-  - abstract (cbn; destruct eqdec; congruence).
-  - abstract (cbn; destruct eqdec; subst; split;
-              intuition; repeat cleanup_step; eauto; congruence).
-  - abstract (cbn; destruct eqdec; subst; split;
-              intuition; repeat cleanup_step; eauto; congruence).
+  destruct sig as [ | (k1' & k2) sig ].
+  - right.
+  - destruct (eq_dec k1 k1'); subst.
+    + left. eexists. apply MemberHd.
+    + destruct (assoc _ _ _ k1 sig) as [ (k2' & m) | ].
+      * left. eexists. apply MemberTl. eassumption.
+      * right.
 Defined.
 
-Scheme Equality for string.
-Instance StringEnv (V: Type) : Env string V := EqEnv string_eq_dec.
-Instance NatEnv (V: Type) : Env nat V := EqEnv PeanoNat.Nat.eq_dec.
+Section Contexts.
+  Context {K: Type}.
+  Context {V: K -> Type}.
 
-Section EnvRel.
-  Context {K V V': Type} {Env: Env K V}.
-  Context (f: V -> V').
+  Inductive context: forall (sig: list K), Type :=
+  | CtxEmpty: context []
+  | CtxCons {sig} (k: K) (v: V k) (ctx: context sig): context (k :: sig).
 
-  Definition env_related (Gamma: fenv K V') (gamma: env_t Env) :=
-    (forall var v, getenv gamma var = Some v -> Gamma var (f v)) /\
-    (forall var, getenv gamma var = None -> forall tau, not (Gamma var tau)).
-
-  Lemma env_related_putenv:
-    forall (Gamma: fenv K V') (gamma: env_t _)
-      (k: K) (v': V') (v: V),
-      f v = v' ->
-      env_related Gamma gamma ->
-      env_related (fenv_add Gamma k v') (putenv gamma k v).
-  Proof.
-    unfold env_related; cbn. intros * ? (H & H') **.
-    split; intros; [
-      pose proof (and_fst (get_put_Some _ _ _ _ _) ltac:(eassumption)) |
-      pose proof (and_fst (get_put_None _ _ _ _) ltac:(eassumption))
-    ]; firstorder (subst; eauto).
-  Qed.
-
-  Lemma env_related_getenv_Some:
-    forall (Gamma: fenv K V') (k: K) (gamma: env_t _),
-      env_related Gamma gamma ->
-      forall v: V,
-        getenv gamma k = Some v ->
-        Gamma k (f v).
-  Proof. firstorder. Qed.
-
-  Lemma env_related_getenv_None:
-    forall (Gamma: fenv K V') (k: K) (gamma: env_t _),
-      env_related Gamma gamma ->
-      getenv gamma k = None ->
-      forall v', Gamma k v' -> False.
-  Proof. firstorder. Qed.
-
-  Definition tenv_of_env (ev: env_t Env): fenv K V'.
-    refine {| fn k v' := exists v, getenv ev k = Some v /\ v' = f v |}.
-    abstract (intros * (? & Heq & Hfeq) (? & Heq' & Hfeq'); subst;
-              rewrite Heq in Heq'; inversion Heq'; eauto).
+  Definition cdestruct {sig} (ctx: context sig)
+    : match sig return context sig -> Type with
+      | [] => fun ctx => ctx = CtxEmpty
+      | k :: sig => fun ctx => { vs: V k * context sig | ctx = CtxCons k (fst vs) (snd vs) }
+      end ctx.
+    destruct ctx.
+    - reflexivity.
+    - exists (v, ctx); reflexivity.
   Defined.
 
-  Lemma tenv_of_env_related :
-    forall (ev: env_t Env),
-      env_related (tenv_of_env ev) ev.
+  Fixpoint ccreate (sig: list K) (f: forall k, V k) : context sig :=
+    match sig with
+    | nil => CtxEmpty
+    | cons h t => CtxCons h (f h) (ccreate t f)
+    end.
+
+  Fixpoint cassoc {sig} {k} (m: member k sig)
+           (ctx: context sig) {struct m} : V k.
   Proof.
-    intros; unfold env_related, tenv_of_env, not; cbn; split.
-    - firstorder.
-    - intros * Heq * Hex; rewrite Heq in Hex;
-        firstorder discriminate.
-  Qed.
+    destruct m; inversion ctx; subst; eauto.
+  Defined.
 
-  Lemma tenv_of_env_nil :
-    env_related fenv_nil env_nil.
-    unfold env_related, fenv_nil; cbn; split; intros.
-    - rewrite getenv_nil in H; discriminate.
-    - tauto.
-  Qed.
-End EnvRel.
+  Fixpoint creplace {sig} {k} (m: member k sig) (v: V k)
+           (ctx: context sig) {struct m} : context sig.
+    destruct m.
+    - destruct (cdestruct ctx) as (vtl & H).
+      eapply (CtxCons k v (snd vtl)).
+    - destruct (cdestruct ctx) as (vtl & H).
+      eapply (CtxCons k' (fst vtl) (creplace sig k m v (snd vtl))).
+  Defined.
 
-Section FEnvRel.
-  Context {K V: Type} {Env: Env K V}.
-
-  Definition fenv_related (Gamma: fenv K V) (gamma: env_t Env) :=
-    forall var v, Gamma var v <-> getenv gamma var = Some v.
-
-  Lemma fenv_related_putenv:
-    forall (Gamma: fenv K V) (gamma: env_t _)
-      (k: K) (v: V),
-      fenv_related Gamma gamma ->
-      fenv_related (fenv_add Gamma k v) (putenv gamma k v).
+  Lemma cassoc_creplace_eq {sig} :
+    forall (ctx: context sig) {k} (m: member k sig) (v: V k),
+      cassoc m (creplace m v ctx) = v.
   Proof.
-    unfold fenv_related; cbn; intros * H **.
-    rewrite get_put_Some, <- H.
-    reflexivity.
+    induction m; cbn; intros.
+    - destruct (cdestruct ctx); cbn. reflexivity.
+    - destruct (cdestruct ctx) as (vtl & Heq); cbn.
+      rewrite IHm; reflexivity.
   Qed.
 
-  Lemma fenv_related_getenv_Some:
-    forall (Gamma: fenv K V) (k: K) (gamma: env_t _),
-      fenv_related Gamma gamma ->
-      forall v: V,
-        Gamma k v -> getenv gamma k = Some v.
-  Proof. firstorder. Qed.
-
-  Lemma fenv_related_getenv_None:
-    forall (Gamma: fenv K V) (k: K) (gamma: env_t _),
-      fenv_related Gamma gamma ->
-      (forall v', Gamma k v' -> False) ->
-      getenv gamma k = None.
-  Proof. firstorder.
-     destruct getenv eqn:Heq.
-     - apply H in Heq; exfalso; eauto.
-     - reflexivity.
-  Qed.
-
-  Lemma tenv_of_env_frelated :
-    forall (ev: env_t Env),
-      fenv_related (tenv_of_env id ev) ev.
+  Lemma cassoc_creplace_neq {sig} :
+    forall (ctx: context sig) {k k'} (m: member k sig) (m': member k' sig) (v: V k),
+      k <> k' ->
+      cassoc m' (creplace m v ctx) = cassoc m' ctx.
   Proof.
-    intros; unfold fenv_related, tenv_of_env, id; cbn; firstorder (subst; eauto).
+    induction m; cbn; intros.
+    - destruct (cdestruct ctx) as (vtl & Heq); cbn; subst.
+      destruct (mdestruct m') as [ (eqn & Heq) | (m'' & Heq)]; subst; cbn in *; subst; cbn.
+      + congruence.
+      + reflexivity.
+    - destruct (cdestruct ctx) as (vtl & Heq); cbn; subst.
+      destruct (mdestruct m') as [ (eqn & Heq) | (m'' & Heq)]; subst; cbn in *; subst; cbn.
+      + reflexivity.
+      + cbn. rewrite IHm; eauto.
   Qed.
-End FEnvRel.
+End Contexts.
 
-Lemma fenv_le_refl {Key Value: Type}:
-  forall (cmp: _ -> _ -> Prop) (Gamma : fenv Key Value),
-    (forall x, cmp x x) ->
-    fenv_le cmp Gamma Gamma.
-Proof.
-  firstorder.
-Qed.
+Arguments context {_}.
 
-Hint Resolve fenv_le_refl : types.
+Notation esig K := (forall k: K, Type).
 
-Lemma fenv_add_increasing {Key Value: Type}:
-  forall (cmp: _ -> _ -> Prop) (Gamma1 : fenv Key Value) (var : Key) (tau tau' : Value) (Gamma2 : fenv Key Value),
-    cmp tau tau' ->
-    fenv_le cmp Gamma1 Gamma2 ->
-    fenv_le cmp (fenv_add Gamma1 var tau) (fenv_add Gamma2 var tau').
-Proof.
-  unfold fenv_le, fenv_add; simpl; firstorder (subst; eauto with types).
-Qed.
+Record Env {K: Type}  :=
+  { env_t: forall (V: esig K), Type;
+    getenv: forall {V: esig K}, env_t V -> forall k, V k;
+    putenv: forall {V: esig K}, env_t V -> forall k, V k -> env_t V;
+    create: forall {V: esig K}, forall (fn: forall k : K, V k), env_t V;
+    get_put_eq: forall {V: esig K} (ev: env_t V) k v, getenv (putenv ev k v) k = v;
+    get_put_neq: forall {V: esig K} (ev: env_t V) k k' v, k <> k' -> getenv (putenv ev k v) k' = getenv ev k';
+    fold_right: forall {V: esig K}, forall {T} (fn: forall k, V k -> T -> T) (ev: env_t V) (t0: T), T }.
+Arguments Env: clear implicits.
 
-Hint Resolve fenv_add_increasing : types.
+Class FiniteType {T} :=
+  { finite_elems: list T;
+    finite_nodup: List.NoDup finite_elems;
+    finite_index: forall t: T, member t finite_elems }.
+Arguments FiniteType: clear implicits.
+
+Definition ContextEnv {K} `{FiniteType K}: Env K.
+  unshelve refine {| env_t V := context V finite_elems;
+                     getenv {V} ctx k := cassoc (finite_index k) ctx;
+                     putenv {V} ctx k v := creplace (finite_index k) v ctx;
+                     create {V} fn := ccreate finite_elems fn;
+                     fold_right {V T} (f: forall k: K, V k -> T -> T) ctx (t0: T) :=
+                       List.fold_right (fun (k: K) (t: T) => f k (cassoc (finite_index k) ctx) t) t0 finite_elems |}.
+  - intros; apply cassoc_creplace_eq.
+  - intros; apply cassoc_creplace_neq; eassumption.
+Defined.
+
+Ltac FiniteType_t :=
+  lazymatch goal with
+  | [  |- FiniteType ?T ] =>
+    econstructor;
+      repeat lazymatch goal with
+             | [  |- forall _: _, member _ _ ] => let t := fresh "t" in intros t; destruct t
+             | [  |- member ?r (_ :: _) ] => apply MemberTl
+             | [  |- member ?r ?l ] => is_evar l; apply MemberHd
+             | _ => idtac
+             end;
+      match goal with
+      | [  |- List.NoDup _ ] => repeat econstructor
+      | _ => fail 2 "Could not prove finiteness of type" T
+      end;
+      match goal with
+      | [  |- ~ List.In _ _ ] => solve [cbv; intuition discriminate]
+      | _ => fail 2 "Could not prove side conditions for finiteness of type" T
+      end
+  end.
+
+Hint Extern 2 (FiniteType _) => FiniteType_t : typeclass_instances.
+
+(* Create HintDb types discriminated. *)
+
+(* Hint Extern 1 => unfold not in *: types. *)
+
+(* Record fenv {Key Value: Type} := *)
+(*   { fn :> Key -> Value -> Prop; *)
+(*     uniq: forall k v v', fn k v -> fn k v' -> v = v' }. *)
+
+(* Arguments fenv: clear implicits. *)
+(* Hint Resolve @uniq : types. *)
+
+(* Definition fenv_nil {Key Value: Type} : fenv Key Value := *)
+(*   {| fn k v := False; *)
+(*      uniq := ltac:(cbv in *; tauto) |}. *)
+
+(* Definition fenv_add {Key Value: Type} (env: fenv Key Value) (k: Key) (v: Value) : fenv Key Value. *)
+(*   refine {| fn := (fun k' v' => (k = k' /\ v = v') \/ (k <> k' /\ env.(fn) k' v')) |}; *)
+(*     abstract (destruct env; intuition (subst; eauto with types)). *)
+(* Defined. *)
+
+(* Definition fenv_le {Key Value: Type} (cmp : Value -> Value -> Prop) (Gamma Gamma': fenv Key Value) := *)
+(*   forall k v, Gamma k v -> exists v', Gamma' k v' /\ cmp v v'. *)
+
+(* Class Env {K R: Type}: Type := *)
+(*   { env_t: Type; *)
+(*     env_nil: env_t; *)
+(*     getenv: env_t -> K -> option R; *)
+(*     putenv: env_t -> K -> R -> env_t; *)
+(*     getenv_nil: forall k, getenv env_nil k = None; *)
+(*     get_put_eq: forall ev k v, getenv (putenv ev k v) k = Some v; *)
+(*     get_put_neq: forall ev k k' v, k <> k' -> getenv (putenv ev k v) k' = getenv ev k'; *)
+(*     get_put_Some: forall ev k k' v v', *)
+(*         getenv (putenv ev k v) k' = Some v' <-> *)
+(*         k = k' /\ v = v' \/ k <> k' /\ getenv ev k' = Some v'; *)
+(*     get_put_None: forall ev k k' v, *)
+(*         getenv (putenv ev k v) k' = None <-> *)
+(*         k <> k' /\ getenv ev k' = None *)
+(*   }. *)
+(* Arguments Env : clear implicits. *)
+(* Arguments env_t {_ _}. *)
+
+(* Instance EqEnv {K R: Type} (eqdec: forall k k': K, {k = k'} + {k <> k'}) : Env K R. *)
+(* Proof. *)
+(*   refine ({| env_t := list (K * R); *)
+(*              env_nil := nil; *)
+(*              getenv e k := *)
+(*                match List.find (fun '(k', v) => if eqdec k k' then true else false) e with *)
+(*                | Some (_, v) => Some v *)
+(*                | None => None *)
+(*                end; *)
+(*              putenv e k v := cons (k, v) e |}); intros. *)
+(*   - abstract (reflexivity). *)
+(*   - abstract (cbn; destruct eqdec; congruence). *)
+(*   - abstract (cbn; destruct eqdec; congruence). *)
+(*   - abstract (cbn; destruct eqdec; subst; split; *)
+(*               intuition; repeat cleanup_step; eauto; congruence). *)
+(*   - abstract (cbn; destruct eqdec; subst; split; *)
+(*               intuition; repeat cleanup_step; eauto; congruence). *)
+(* Defined. *)
+
+(* Scheme Equality for string. *)
+(* Instance StringEnv (R: Type) : Env string R := EqEnv string_eq_dec. *)
+(* Instance NatEnv (R: Type) : Env nat R := EqEnv PeanoNat.Nat.eq_dec. *)
+
+(* Section EnvRel. *)
+(*   Context {K R R': Type} {Env: Env K R}. *)
+(*   Context (f: R -> R'). *)
+
+(*   Definition env_related (Gamma: fenv K R') (gamma: env_t Env) := *)
+(*     (forall var v, getenv gamma var = Some v -> Gamma var (f v)) /\ *)
+(*     (forall var, getenv gamma var = None -> forall tau, not (Gamma var tau)). *)
+
+(*   Lemma env_related_putenv: *)
+(*     forall (Gamma: fenv K R') (gamma: env_t _) *)
+(*       (k: K) (v': R') (v: R), *)
+(*       f v = v' -> *)
+(*       env_related Gamma gamma -> *)
+(*       env_related (fenv_add Gamma k v') (putenv gamma k v). *)
+(*   Proof. *)
+(*     unfold env_related; cbn. intros * ? (H & H') **. *)
+(*     split; intros; [ *)
+(*       pose proof (and_fst (get_put_Some _ _ _ _ _) ltac:(eassumption)) | *)
+(*       pose proof (and_fst (get_put_None _ _ _ _) ltac:(eassumption)) *)
+(*     ]; firstorder (subst; eauto). *)
+(*   Qed. *)
+
+(*   Lemma env_related_getenv_Some: *)
+(*     forall (Gamma: fenv K R') (k: K) (gamma: env_t _), *)
+(*       env_related Gamma gamma -> *)
+(*       forall v: R, *)
+(*         getenv gamma k = Some v -> *)
+(*         Gamma k (f v). *)
+(*   Proof. firstorder. Qed. *)
+
+(*   Lemma env_related_getenv_None: *)
+(*     forall (Gamma: fenv K R') (k: K) (gamma: env_t _), *)
+(*       env_related Gamma gamma -> *)
+(*       getenv gamma k = None -> *)
+(*       forall v', Gamma k v' -> False. *)
+(*   Proof. firstorder. Qed. *)
+
+(*   Definition tenv_of_env (ev: env_t Env): fenv K R'. *)
+(*     refine {| fn k v' := exists v, getenv ev k = Some v /\ v' = f v |}. *)
+(*     abstract (intros * (? & Heq & Hfeq) (? & Heq' & Hfeq'); subst; *)
+(*               rewrite Heq in Heq'; inversion Heq'; eauto). *)
+(*   Defined. *)
+
+(*   Lemma tenv_of_env_related : *)
+(*     forall (ev: env_t Env), *)
+(*       env_related (tenv_of_env ev) ev. *)
+(*   Proof. *)
+(*     intros; unfold env_related, tenv_of_env, not; cbn; split. *)
+(*     - firstorder. *)
+(*     - intros * Heq * Hex; rewrite Heq in Hex; *)
+(*         firstorder discriminate. *)
+(*   Qed. *)
+
+(*   Lemma tenv_of_env_nil : *)
+(*     env_related fenv_nil env_nil. *)
+(*     unfold env_related, fenv_nil; cbn; split; intros. *)
+(*     - rewrite getenv_nil in H; discriminate. *)
+(*     - tauto. *)
+(*   Qed. *)
+(* End EnvRel. *)
+
+(* Section FEnvRel. *)
+(*   Context {K R: Type} {Env: Env K R}. *)
+
+(*   Definition fenv_related (Gamma: fenv K R) (gamma: env_t Env) := *)
+(*     forall var v, Gamma var v <-> getenv gamma var = Some v. *)
+
+(*   Lemma fenv_related_putenv: *)
+(*     forall (Gamma: fenv K R) (gamma: env_t _) *)
+(*       (k: K) (v: R), *)
+(*       fenv_related Gamma gamma -> *)
+(*       fenv_related (fenv_add Gamma k v) (putenv gamma k v). *)
+(*   Proof. *)
+(*     unfold fenv_related; cbn; intros * H **. *)
+(*     rewrite get_put_Some, <- H. *)
+(*     reflexivity. *)
+(*   Qed. *)
+
+(*   Lemma fenv_related_getenv_Some: *)
+(*     forall (Gamma: fenv K R) (k: K) (gamma: env_t _), *)
+(*       fenv_related Gamma gamma -> *)
+(*       forall v: R, *)
+(*         Gamma k v -> getenv gamma k = Some v. *)
+(*   Proof. firstorder. Qed. *)
+
+(*   Lemma fenv_related_getenv_None: *)
+(*     forall (Gamma: fenv K R) (k: K) (gamma: env_t _), *)
+(*       fenv_related Gamma gamma -> *)
+(*       (forall v', Gamma k v' -> False) -> *)
+(*       getenv gamma k = None. *)
+(*   Proof. firstorder. *)
+(*      destruct getenv eqn:Heq. *)
+(*      - apply H in Heq; exfalso; eauto. *)
+(*      - reflexivity. *)
+(*   Qed. *)
+
+(*   Lemma tenv_of_env_frelated : *)
+(*     forall (ev: env_t Env), *)
+(*       fenv_related (tenv_of_env id ev) ev. *)
+(*   Proof. *)
+(*     intros; unfold fenv_related, tenv_of_env, id; cbn; firstorder (subst; eauto). *)
+(*   Qed. *)
+(* End FEnvRel. *)
+
+(* Lemma fenv_le_refl {Key Value: Type}: *)
+(*   forall (cmp: _ -> _ -> Prop) (Gamma : fenv Key Value), *)
+(*     (forall x, cmp x x) -> *)
+(*     fenv_le cmp Gamma Gamma. *)
+(* Proof. *)
+(*   firstorder. *)
+(* Qed. *)
+
+(* Hint Resolve fenv_le_refl : types. *)
+
+(* Lemma fenv_add_increasing {Key Value: Type}: *)
+(*   forall (cmp: _ -> _ -> Prop) (Gamma1 : fenv Key Value) (var : Key) (tau tau' : Value) (Gamma2 : fenv Key Value), *)
+(*     cmp tau tau' -> *)
+(*     fenv_le cmp Gamma1 Gamma2 -> *)
+(*     fenv_le cmp (fenv_add Gamma1 var tau) (fenv_add Gamma2 var tau'). *)
+(* Proof. *)
+(*   unfold fenv_le, fenv_add; simpl; firstorder (subst; eauto with types). *)
+(* Qed. *)
+
+(* Hint Resolve fenv_add_increasing : types. *)
 
