Syntax.v
@@ -1,56 +1,30 @@
-Inductive Level :=
+Require Import SGA.Common.
+
+Inductive Port :=
   P0 | P1.
 
-Notation bits := (list bool).
+Section Syntax.
+  Context {var_t reg_t fn_t: Type}.
 
-Inductive rule {TVar TFn} :=
-| Bind (var: TVar) (expr: rule) (body: rule)
-| Var (var: TVar)
-| Skip
-| Const (cst: bits)
-| If (cond: rule) (tbranch: rule) (fbranch: rule)
-| Fail
-| Read (level: Level) (idx: nat)
-| Write (level: Level) (idx: nat) (value: rule)
-| Call (fn: TFn) (args: list rule).
+  Inductive uexpr :=
+  | UVar (var: var_t)
+  | UConst {n} (cst: bits n)
+  | URead (port: Port) (idx: reg_t)
+  | UCall (fn: fn_t) (arg1: uexpr) (arg2: uexpr).
 
-Arguments rule : clear implicits.
+  Inductive urule  :=
+  | USkip
+  | UFail
+  | USeq (r1 r2: urule)
+  | UBind (v: var_t) (ex: uexpr) (body: urule)
+  | UIf (cond: uexpr) (tbranch: urule) (fbranch: urule)
+  | UWrite (port: Port) (idx: reg_t) (value: uexpr).
 
-Inductive scheduler {TVar TFn} :=
-| Done
-| Try (r: rule TVar TFn) (s1 s2: scheduler).
+  Inductive uscheduler :=
+  | UDone
+  | UTry (r: urule) (s1 s2: uscheduler).
+End Syntax.
 
-Arguments scheduler : clear implicits.
-
-Require Import List.
-
-(* Better induction principle *)
-Definition rule_ind' {TVar TFn : Type} (P : rule TVar TFn -> Prop)
-           (f : forall (var : TVar) (expr : rule TVar TFn),
-               P expr -> forall body : rule TVar TFn, P body -> P (Bind var expr body))
-           (f0 : forall var : TVar, P (Var var)) (f1 : P Skip) (f2 : forall cst : bits, P (Const cst))
-           (f3 : forall cond : rule TVar TFn,
-               P cond ->
-               forall tbranch : rule TVar TFn,
-                 P tbranch -> forall fbranch : rule TVar TFn, P fbranch -> P (If cond tbranch fbranch))
-           (f4 : P Fail) (f5 : forall (level : Level) (idx : nat), P (Read level idx))
-           (f6 : forall (level : Level) (idx : nat) (value : rule TVar TFn), P value -> P (Write level idx value))
-           (f7: forall (fn : TFn) (args : list (rule TVar TFn)),
-               List.Forall P args ->
-               P (Call fn args)) : forall r, P r.
-  refine (fix F (r : rule TVar TFn) : P r :=
-            match r as r0 return (P r0) with
-            | Bind var expr body => f var expr (F expr) body (F body)
-            | Var var => f0 var
-            | Skip => f1
-            | Const cst => f2 cst
-            | If cond tbranch fbranch => f3 cond (F cond) tbranch (F tbranch) fbranch (F fbranch)
-            | Fail => f4
-            | Read level idx => f5 level idx
-            | Write level idx value => f6 level idx value (F value)
-            | Call fn args => f7 fn args _
-            end).
-  revert args.
-  fix fargs 1.
-  destruct args; cbn; econstructor; eauto.
-Defined.
+Arguments uexpr : clear implicits.
+Arguments urule : clear implicits.
+Arguments uscheduler : clear implicits.
