TypeInference.v
@@ -1,242 +1,278 @@
-Require Import SGA.Common SGA.Syntax SGA.Environments SGA.Types SGA.Typechecking.
+Require Import SGA.Common SGA.Environments SGA.Syntax SGA.Types.
+Require Import Coq.Lists.List.
+Import ListNotations.
 
 Section TypeInference.
-  Context {TVar TFn: Type}.
-  Context {GammaEnv: Env TVar type}.
-  Context {RegEnv: Env nat nat}.
-  Context (SigmaEnv: Env TFn ExternalSignature).
+  Context {var_t reg_t fn_t: Type}.
+  Context {var_t_eq_dec: EqDec var_t}.
 
-  Context (Sigma: SigmaEnv.(env_t)).
-  Context (V: RegEnv.(env_t)).
+  Context (R: reg_t -> type).
+  Context (Sigma: fn_t -> ExternalSignature).
 
   Open Scope bool_scope.
 
-  Definition type_le_dec tau1 tau2:
-    { type_le tau1 tau2 } + { ~ type_le tau1 tau2 }.
-  Proof.
-    destruct tau1, tau2; try destruct (PeanoNat.Nat.eq_dec n n0);
-      cbn; repeat match goal with
-                  | [ H: bit_t _ = bit_t _ |- _ ] => inversion H; subst; clear H
-                  | _ => discriminate
-                  | _ => solve [eauto with types]
-                  | _ => right; inversion 1
-                  end.
-  Defined.
+  Notation uexpr := (uexpr var_t reg_t fn_t).
+  Notation urule := (urule var_t reg_t fn_t).
+  Notation uscheduler := (uscheduler var_t reg_t fn_t).
 
-  Arguments type_le_dec: simpl never.
+  Notation expr := (expr var_t R Sigma).
+  Notation rule := (rule var_t R Sigma).
+  Notation scheduler := (scheduler var_t R Sigma).
 
-  Fixpoint infer_maxtype
-           (Gamma: GammaEnv.(env_t))
-           (r: rule TVar TFn)
-    : option type :=
-    match r with
-    | Bind var expr body =>
-      opt_bind (infer_maxtype Gamma expr) (fun etau =>
-      infer_maxtype (putenv Gamma var etau) body)
-    | Var var => getenv Gamma var
-    | Skip => Some unit_t
-    | Const cst => Some (bit_t (List.length cst))
-    | If cond tbranch fbranch =>
-      opt_bind (infer_maxtype Gamma cond) (fun ctau =>
-      if type_le_dec (bit_t 1) ctau then
-        opt_bind (infer_maxtype Gamma tbranch) (fun ttau =>
-        opt_bind (infer_maxtype Gamma fbranch) (fun ftau =>
-        if type_le_dec ftau ttau then Some ftau
-        else if type_le_dec ttau ftau then Some ttau
-             else None))
-      else None)
-    | Fail => Some any_t
-    | Read level idx =>
-      opt_bind (getenv V idx) (fun sz => Some (bit_t sz))
-    | Write level idx value =>
-      opt_bind (infer_maxtype Gamma value) (fun vtau =>
-      opt_bind (getenv V idx) (fun sz =>
-      if type_le_dec (bit_t sz) vtau then Some unit_t
-      else None))
-    | Call fn args =>
-      opt_bind (getenv Sigma fn) (fun '(FunSig argSizes retSize) =>
-      if (PeanoNat.Nat.eq_dec (List.length args) (List.length argSizes)) then
-        if (fold_right2 (fun arg argSize acc =>
-                          acc && match infer_maxtype Gamma arg with
-                                 | Some tau => if type_le_dec (bit_t argSize) tau then true else false
-                                 | None => false
-                                 end)
-                       true args argSizes) then
-          Some (bit_t retSize)
-        else None
-      else None)
-    end.
+  Notation "` x" := (projT1 x) (at level 0).
+  Notation "`` x" := (projT2 x) (at level 0).
 
-  Hint Resolve (@env_related_putenv _ _ _ GammaEnv): types.
-  Hint Resolve fenv_related_putenv: types.
-  Hint Constructors HasType : types.
-  Hint Extern 0 => unfold id : types.
+  Section Expr.
+    Context (sig: tsig var_t).
 
-  Ltac t :=
-    repeat match goal with
-           | _ => reflexivity
-           | _ => progress cleanup_step
-           | [ H: opt_bind ?x _ = Some _ |- _ ] =>
-             destruct x eqn:?; cbn in H; [ | discriminate]
-           | [ H: match ?x with _ => _ end = Some _ |- _ ] =>
-             destruct x eqn:?
-           | [ H: env_related (Env := ?Env) ?f ?tenv ?env,
-                  H': getenv ?env ?k = Some ?v |- _ ] =>
-             pose_once (and_fst H k v) H'
-           | [ H: forall Gamma gamma tau, _ -> _ = Some _ -> _,
-                 H': infer_maxtype ?Gamma ?r = Some ?tau |- _ ] =>
-             specialize (H Gamma _ tau ltac:(eauto with types) H')
-           | [ H: MaxType ?V ?Sigma ?Gamma ?r ?tau |- _ ] =>
-             pose_once (MaxType_HasType V Sigma Gamma r tau) H
-           | _ => solve [econstructor] || econstructor; solve [eauto 5 with types]
-           end.
+    Definition cast_expr
+               {tau1} tau2 (e: expr sig tau1)
+      : option (expr sig tau2).
+    Proof.
+      destruct (eq_dec tau1 tau2); subst.
+      - exact (Some e).
+      - exact None.
+    Defined.
 
-   Lemma infer_maxtype_correct_call:
-    forall sigma v,
-      env_related id v V ->
-      env_related id sigma Sigma ->
-     forall args argSizes,
-       length args = length argSizes ->
-       forall Gamma gamma,
-         env_related id gamma Gamma ->
-         List.Forall
-           (fun r : rule TVar TFn =>
-              forall Gamma gamma tau,
-                env_related id gamma Gamma -> infer_maxtype Gamma r = Some tau -> MaxType v sigma gamma r tau) args ->
-         fold_right2
-           (fun arg argSize acc =>
-              acc &&
-                  match infer_maxtype Gamma arg with
-                  | Some tau => if type_le_dec (bit_t argSize) tau then true else false
-                  | None => false
-                  end) true args argSizes = true ->
-         fold_right2
-           (fun (arg : rule TVar TFn) (argSize : nat) (acc : Prop) => acc /\ HasType v sigma gamma arg (bit_t argSize))
-           True args argSizes.
-   Proof.
-     induction args; destruct argSizes; cbn in *;
-       inversion 1; intros ? ? ?; inversion 1; subst; intros Heq.
-     - eauto.
-     - destruct infer_maxtype eqn:?;
-         apply andb_prop in Heq; repeat cleanup_step.
-       destruct type_le_dec; try discriminate.
-       eauto using MaxType_HasType.
-   Qed.
+    Notation EX Px := (existT _ _ Px).
 
-  Lemma infer_maxtype_correct :
-    forall sigma v,
-      env_related id v V ->
-      env_related id sigma Sigma ->
-      forall (r: rule TVar TFn) (Gamma: GammaEnv.(env_t)) gamma (tau: type),
-        env_related id gamma Gamma ->
-        infer_maxtype Gamma r = Some tau ->
-        MaxType v sigma gamma r tau.
-  Proof.
-    induction r using rule_ind'; cbn; intros; t.
-
-    econstructor; eauto.
-    eapply fold_right2_forall2;
-      eauto using infer_maxtype_correct_call.
-  Qed.
-
-  Lemma forall2_cons_inv {A B} (P: A -> B -> Prop) :
-    forall a b la lb,
-      forall2 P (a :: la) (b :: lb) ->
-      P a b /\ forall2 P la lb.
-  Proof.
-    intros * H; apply forall2_fold_right2 in H; destruct H as (H & ?).
-    apply fold_right2_forall2 in H; intuition.
-  Qed.
-
-  Ltac tcomplete_step :=
-    match goal with
-    | _ => progress subst
-    | _ => progress intros
-    | [ H: fn ?gamma ?k ?v, H': fenv_related ?gamma ?Gamma |- _ ] =>
-      try pose_once H' k v;
-      match goal with
-      | [ H'': fn gamma k v <-> getenv Gamma k = Some v |- _ ] =>
-        pose_once (and_fst H'') H
-      end
-    | [ H: HasType _ _ _ _ _ |- _ ] =>
-      apply HasType_MaxType in H; destruct H as (? & ? & ?)
-    | [ H: ?x = Some _ |- opt_bind ?x _ = _ ] =>
-      rewrite H; cbn
-    | [ H: (forall _ _ , _ -> forall _, _ -> infer_maxtype _ ?r  = Some _)  |-
-        opt_bind (infer_maxtype _ ?r) _ = Some _ ] =>
-      erewrite H by eauto with types; cbn
-    | [ H: type_le ?x ?y |- context[type_le_dec ?x ?y] ] =>
-      destruct type_le_dec; try tauto
-    | _ => cleanup_step
-    end.
-
-  Lemma infer_maxtype_complete_call:
-    forall (sigma : fenv TFn ExternalSignature) (v : fenv nat nat) (args : list (rule TVar TFn)) argSizes,
-      length args = length argSizes ->
-      List.Forall
-        (fun r : rule TVar TFn =>
-           forall (gamma : fenv TVar type) (tau : type),
-             MaxType v sigma gamma r tau ->
-             forall Gamma : env_t GammaEnv, fenv_related gamma Gamma -> infer_maxtype Gamma r = Some tau) args ->
-      forall (gamma : fenv TVar type) (Gamma : env_t GammaEnv),
-        forall2 (fun (arg : rule TVar TFn) (argSize : nat) => HasType v sigma gamma arg (bit_t argSize)) args argSizes ->
-        fenv_related gamma Gamma ->
-        forall b : bool,
-          fold_right2
-            (fun (arg : rule TVar TFn) (argSize : nat) (acc : bool) =>
-             acc &&
-             match infer_maxtype Gamma arg with
-             | Some tau0 => if type_le_dec (bit_t argSize) tau0 then true else false
-             | None => false
-             end) b args argSizes = b.
-  Proof.
-    induction args; cbn; destruct argSizes; inversion 1; intros HForall * Hforall2 **.
-    - reflexivity.
-    - inversion HForall as [ | x l Hinfer HForall']; subst.
-
-      apply forall2_cons_inv in Hforall2.
-
-      repeat tcomplete_step.
-      erewrite Hinfer; eauto.
-      repeat tcomplete_step.
-      rewrite Bool.andb_true_r.
-      eauto.
-  Qed.
-
-  Lemma infer_maxtype_complete :
-    forall sigma v,
-      fenv_related v V ->
-      fenv_related sigma Sigma ->
-      forall (r: rule TVar TFn) gamma (tau: type),
-        MaxType v sigma gamma r tau ->
-        forall (Gamma: GammaEnv.(env_t)),
-        fenv_related gamma Gamma ->
-        infer_maxtype Gamma r = Some tau.
-  Proof.
-    induction r using rule_ind'; cbn; inversion 1;
-      repeat tcomplete_step; eauto using f_equal with types.
-
-    - destruct PeanoNat.Nat.eq_dec; try tauto.
-      erewrite infer_maxtype_complete_call; eauto.
-  Qed.
-
-  Theorem TypeInference :
-    forall Gamma (r: rule TVar TFn),
-      match infer_maxtype Gamma r with
-      | Some tau => HasType (tenv_of_env id V) (tenv_of_env id Sigma) (tenv_of_env id Gamma) r tau
-      | None => forall tau, not (HasType (tenv_of_env id V) (tenv_of_env id Sigma) (tenv_of_env id Gamma) r tau)
+    Fixpoint type_expr (e: uexpr)
+      : option ({ tau: type & expr sig tau }) :=
+      match e with
+      | UVar var =>
+        let/opt ktau_m := assoc var sig in
+        Some (EX (Var ``ktau_m))
+      | UConst cst => Some (EX (Const cst))
+      | URead port idx => Some (EX (Read port idx))
+      | UCall fn arg1 arg2 =>
+        let/opt arg1' := type_expr arg1 in
+        let/opt arg2' := type_expr arg2 in
+        let/opt arg1' := cast_expr (Sigma fn).(arg1Type) (``arg1') in
+        let/opt arg2' := cast_expr (Sigma fn).(arg2Type) (``arg2') in
+        Some (EX (Call fn arg1' arg2'))
       end.
-  Proof.
-    intros; destruct infer_maxtype eqn:?.
-    - eapply MaxType_HasType.
-      + eapply infer_maxtype_correct;
-          try eapply tenv_of_env_related; eauto.
-      + eauto with types.
-    - intros tau Habs.
-      eapply HasType_MaxType in Habs.
-      destruct Habs as (? & Habs & Hle).
-      eapply infer_maxtype_complete in Habs;
-        try eapply tenv_of_env_frelated.
-      congruence.
-  Qed.
+  End Expr.
+
+  Section Rule.
+    Fixpoint type_rule (sig: tsig var_t)
+             (r: urule) : option (rule sig) :=
+      match r with
+      | USkip => Some Skip
+      | UFail => Some Fail
+      | USeq r1 r2 =>
+        let/opt r1 := type_rule sig r1 in
+        let/opt r2 := type_rule sig r2 in
+        Some (Seq r1 r2)
+      | UBind v ex body =>
+        let/opt ex := type_expr sig ex in
+        let/opt body := type_rule ((v, `ex) :: sig) body in
+        Some (Bind v ``ex body)
+      | UIf cond tbranch fbranch =>
+        let/opt cond := type_expr sig cond in
+        let/opt tbranch := type_rule sig tbranch in
+        let/opt fbranch := type_rule sig fbranch in
+        let/opt cond := cast_expr sig (bits_t 1) (``cond) in
+        Some (If cond tbranch fbranch)
+      | UWrite port idx value =>
+        let/opt value := type_expr sig value in
+        let/opt value := cast_expr sig (R idx) (``value) in
+        Some (Write port idx value)
+      end.
+  End Rule.
+
+  Section Scheduler.
+    Fixpoint type_scheduler (s: uscheduler) : option scheduler :=
+      match s with
+      | UDone =>
+        Some Done
+      | UTry r s1 s2 =>
+        let/opt r := type_rule [] r in
+        let/opt s1 := type_scheduler s1 in
+        let/opt s2 := type_scheduler s2 in
+        Some (Try r s1 s2)
+      end.
+  End Scheduler.
 End TypeInference.
+
+Notation tc R Sigma prog :=
+  ltac:(let tcopt := match type of prog with
+                     | urule _ _ _ => constr:(type_rule R Sigma List.nil prog)
+                     | uscheduler _ _ _ => constr:(type_scheduler R Sigma prog)
+                     end in
+        let tcopt := (eval cbn in tcopt) in
+        let tcterm := (eval cbn in (must tcopt)) in
+        exact tcterm) (only parsing).
+
+(*   Hint Resolve (@env_related_putenv _ _ _ GammaEnv): types. *)
+(*   Hint Resolve fenv_related_putenv: types. *)
+(*   Hint Constructors HasType : types. *)
+(*   Hint Extern 0 => unfold id : types. *)
+
+(*   Ltac t := *)
+(*     repeat match goal with *)
+(*            | _ => reflexivity *)
+(*            | _ => progress cleanup_step *)
+(*            | [ H: opt_bind ?x _ = Some _ |- _ ] => *)
+(*              destruct x eqn:?; cbn in H; [ | discriminate] *)
+(*            | [ H: match ?x with _ => _ end = Some _ |- _ ] => *)
+(*              destruct x eqn:? *)
+(*            | [ H: env_related (Env := ?Env) ?f ?tenv ?env, *)
+(*                   H': getenv ?env ?k = Some ?v |- _ ] => *)
+(*              pose_once (and_fst H k v) H' *)
+(*            | [ H: forall Gamma gamma tau, _ -> _ = Some _ -> _, *)
+(*                  H': type_expr ?Gamma ?r = Some ?tau |- _ ] => *)
+(*              specialize (H Gamma _ tau ltac:(eauto with types) H') *)
+(*            | [ H: MaxType ?R ?Sigma ?Gamma ?r ?tau |- _ ] => *)
+(*              pose_once (MaxType_HasType R Sigma Gamma r tau) H *)
+(*            | _ => solve [econstructor] || econstructor; solve [eauto 5 with types] *)
+(*            end. *)
+
+(*    Lemma type_expr_correct_call: *)
+(*     forall sigma v, *)
+(*       env_related id v R -> *)
+(*       env_related id sigma Sigma -> *)
+(*      forall args argSizes, *)
+(*        length args = length argSizes -> *)
+(*        forall Gamma gamma, *)
+(*          env_related id gamma Gamma -> *)
+(*          List.Forall *)
+(*            (fun r : rule var_t fn_t => *)
+(*               forall Gamma gamma tau, *)
+(*                 env_related id gamma Gamma -> type_expr Gamma r = Some tau -> MaxType v sigma gamma r tau) args -> *)
+(*          fold_right2 *)
+(*            (fun arg argSize acc => *)
+(*               acc && *)
+(*                   match type_expr Gamma arg with *)
+(*                   | Some tau => if type_le_dec (bits_t argSize) tau then true else false *)
+(*                   | None => false *)
+(*                   end) true args argSizes = true -> *)
+(*          fold_right2 *)
+(*            (fun (arg : rule var_t fn_t) (argSize : nat) (acc : Prop) => acc /\ HasType v sigma gamma arg (bits_t argSize)) *)
+(*            True args argSizes. *)
+(*    Proof. *)
+(*      induction args; destruct argSizes; cbn in *; *)
+(*        inversion 1; intros ? ? ?; inversion 1; subst; intros Heq. *)
+(*      - eauto. *)
+(*      - destruct type_expr eqn:?; *)
+(*          apply andb_prop in Heq; repeat cleanup_step. *)
+(*        destruct type_le_dec; try discriminate. *)
+(*        eauto using MaxType_HasType. *)
+(*    Qed. *)
+
+(*   Lemma type_expr_correct : *)
+(*     forall sigma v, *)
+(*       env_related id v R -> *)
+(*       env_related id sigma Sigma -> *)
+(*       forall (r: rule var_t fn_t) (Gamma: GammaEnv.(env_t)) gamma (tau: type), *)
+(*         env_related id gamma Gamma -> *)
+(*         type_expr Gamma r = Some tau -> *)
+(*         MaxType v sigma gamma r tau. *)
+(*   Proof. *)
+(*     induction r using rule_ind'; cbn; intros; t. *)
+
+(*     econstructor; eauto. *)
+(*     eapply fold_right2_forall2; *)
+(*       eauto using type_expr_correct_call. *)
+(*   Qed. *)
+
+(*   Lemma forall2_cons_inv {A B} (P: A -> B -> Prop) : *)
+(*     forall a b la lb, *)
+(*       forall2 P (a :: la) (b :: lb) -> *)
+(*       P a b /\ forall2 P la lb. *)
+(*   Proof. *)
+(*     intros * H; apply forall2_fold_right2 in H; destruct H as (H & ?). *)
+(*     apply fold_right2_forall2 in H; intuition. *)
+(*   Qed. *)
+
+(*   Ltac tcomplete_step := *)
+(*     match goal with *)
+(*     | _ => progress subst *)
+(*     | _ => progress intros *)
+(*     | [ H: fn ?gamma ?k ?v, H': fenv_related ?gamma ?Gamma |- _ ] => *)
+(*       try pose_once H' k v; *)
+(*       match goal with *)
+(*       | [ H'': fn gamma k v <-> getenv Gamma k = Some v |- _ ] => *)
+(*         pose_once (and_fst H'') H *)
+(*       end *)
+(*     | [ H: HasType _ _ _ _ _ |- _ ] => *)
+(*       apply HasType_MaxType in H; destruct H as (? & ? & ?) *)
+(*     | [ H: ?x = Some _ |- opt_bind ?x _ = _ ] => *)
+(*       rewrite H; cbn *)
+(*     | [ H: (forall _ _ , _ -> forall _, _ -> type_expr _ ?r  = Some _)  |- *)
+(*         opt_bind (type_expr _ ?r) _ = Some _ ] => *)
+(*       erewrite H by eauto with types; cbn *)
+(*     | [ H: type_le ?x ?y |- context[type_le_dec ?x ?y] ] => *)
+(*       destruct type_le_dec; try tauto *)
+(*     | _ => cleanup_step *)
+(*     end. *)
+
+(*   Lemma type_expr_complete_call: *)
+(*     forall (sigma : fenv fn_t ExternalSignature) (v : fenv nat nat) (args : list (rule var_t fn_t)) argSizes, *)
+(*       length args = length argSizes -> *)
+(*       List.Forall *)
+(*         (fun r : rule var_t fn_t => *)
+(*            forall (gamma : fenv var_t type) (tau : type), *)
+(*              MaxType v sigma gamma r tau -> *)
+(*              forall Gamma : env_t GammaEnv, fenv_related gamma Gamma -> type_expr Gamma r = Some tau) args -> *)
+(*       forall (gamma : fenv var_t type) (Gamma : env_t GammaEnv), *)
+(*         forall2 (fun (arg : rule var_t fn_t) (argSize : nat) => HasType v sigma gamma arg (bits_t argSize)) args argSizes -> *)
+(*         fenv_related gamma Gamma -> *)
+(*         forall b : bool, *)
+(*           fold_right2 *)
+(*             (fun (arg : rule var_t fn_t) (argSize : nat) (acc : bool) => *)
+(*              acc && *)
+(*              match type_expr Gamma arg with *)
+(*              | Some tau0 => if type_le_dec (bits_t argSize) tau0 then true else false *)
+(*              | None => false *)
+(*              end) b args argSizes = b. *)
+(*   Proof. *)
+(*     induction args; cbn; destruct argSizes; inversion 1; intros HForall * Hforall2 **. *)
+(*     - reflexivity. *)
+(*     - inversion HForall as [ | x l Hinfer HForall']; subst. *)
+
+(*       apply forall2_cons_inv in Hforall2. *)
+
+(*       repeat tcomplete_step. *)
+(*       erewrite Hinfer; eauto. *)
+(*       repeat tcomplete_step. *)
+(*       rewrite Bool.andb_true_r. *)
+(*       eauto. *)
+(*   Qed. *)
+
+(*   Lemma type_expr_complete : *)
+(*     forall sigma v, *)
+(*       fenv_related v R -> *)
+(*       fenv_related sigma Sigma -> *)
+(*       forall (r: rule var_t fn_t) gamma (tau: type), *)
+(*         MaxType v sigma gamma r tau -> *)
+(*         forall (Gamma: GammaEnv.(env_t)), *)
+(*         fenv_related gamma Gamma -> *)
+(*         type_expr Gamma r = Some tau. *)
+(*   Proof. *)
+(*     induction r using rule_ind'; cbn; inversion 1; *)
+(*       repeat tcomplete_step; eauto using f_equal with types. *)
+
+(*     - destruct PeanoNat.Nat.eq_dec; try tauto. *)
+(*       erewrite type_expr_complete_call; eauto. *)
+(*   Qed. *)
+
+(*   Theorem TypeInference : *)
+(*     forall Gamma (r: rule var_t fn_t), *)
+(*       match type_expr Gamma r with *)
+(*       | Some tau => HasType (tenv_of_env id R) (tenv_of_env id Sigma) (tenv_of_env id Gamma) r tau *)
+(*       | None => forall tau, not (HasType (tenv_of_env id R) (tenv_of_env id Sigma) (tenv_of_env id Gamma) r tau) *)
+(*       end. *)
+(*   Proof. *)
+(*     intros; destruct type_expr eqn:?. *)
+(*     - eapply MaxType_HasType. *)
+(*       + eapply type_expr_correct; *)
+(*           try eapply tenv_of_env_related; eauto. *)
+(*       + eauto with types. *)
+(*     - intros tau Habs. *)
+(*       eapply HasType_MaxType in Habs. *)
+(*       destruct Habs as (? & Habs & Hle). *)
+(*       eapply type_expr_complete in Habs; *)
+(*         try eapply tenv_of_env_frelated. *)
+(*       congruence. *)
+(*   Qed. *)
+(* End TypeInference. *)
